progs/field_mapsto.v
@@ -1,0 +1,255 @@
+Require Import veric.SeparationLogic.
+Require veric.SequentialClight.
+Import SequentialClight.SeqC.CSL.
+
+Local Open Scope logic.
+
+Lemma field_offset_rec_unroll:
+  forall fields0 fld sid fields n,
+    field_offset_rec fld (unroll_composite_fields sid (Tstruct sid fields0 noattr) fields) n =
+    field_offset_rec fld fields n.
+Proof.
+intros. revert n; induction fields; intros; auto.
+unfold unroll_composite_fields, field_offset.
+simpl. if_tac.
+f_equal.
+f_equal.
+change (alignof (unroll_composite  sid (Tstruct sid fields0 noattr) t) = alignof t).
+apply alignof_unroll_composite.
+change (field_offset_rec fld  (unroll_composite_fields sid (Tstruct sid fields0 noattr) fields)
+             (align n (alignof (unroll_composite sid (Tstruct sid fields0 noattr) t)) 
+                          + sizeof (unroll_composite sid (Tstruct sid fields0 noattr) t)) = 
+    field_offset_rec fld fields (align n (alignof t) + sizeof t)).
+rewrite IHfields.
+rewrite alignof_unroll_composite.
+rewrite sizeof_unroll_composite.
+auto.
+Qed.
+
+Lemma field_offset_unroll:
+  forall fields0 fld sid fields,
+    field_offset fld (unroll_composite_fields sid (Tstruct sid fields0 noattr) fields) =
+    field_offset fld fields.
+Proof.
+intros.
+apply field_offset_rec_unroll.
+Qed.
+
+Fixpoint type_of_field (f: fieldlist) (fld: ident) : type :=
+ match f with
+ | Fnil => Tvoid
+ | Fcons i t fl => if eq_dec i fld then t else type_of_field fl fld
+ end.
+
+Definition field_mapsto (sh: Share.t) (t1: type) (fld: ident) (v1 v2: val) : mpred :=
+ match v1, t1 with
+  | Vptr l ofs, Tstruct id fList  att =>
+    let fList' := unroll_composite_fields id t1 fList in
+    let t2 := type_of_field fList' fld in
+     match field_offset fld fList',  access_mode t2 with
+     | Errors.OK delta, By_value ch => 
+          !! (typecheck_val v2 t2 = true) && !!(type_is_volatile t2 = false) &&
+           address_mapsto ch v2 (Share.unrel Share.Lsh sh) (Share.unrel Share.Rsh sh)  (l, Int.unsigned (Int.add ofs (Int.repr delta)))
+     | _, _ => FF
+     end
+  | _, _  => FF
+  end.
+
+Lemma field_mapsto_typecheck_val:
+  forall t fld sh x y id fList att, 
+     t = Tstruct id fList att ->
+     field_mapsto sh t fld x y = 
+               !! (typecheck_val y (type_of_field (unroll_composite_fields id t fList) fld) = true) && field_mapsto sh t fld x y.
+Proof.
+intros. subst.
+apply pred_ext; normalize.
+apply andp_right; auto.
+unfold field_mapsto.
+destruct x; normalize.
+destruct (field_offset fld (unroll_composite_fields id (Tstruct id fList att) fList)); normalize.
+destruct (access_mode
+    (type_of_field (unroll_composite_fields id (Tstruct id fList att) fList) fld)); normalize.
+Qed.
+
+Lemma field_mapsto_nonnull:  forall t fld sh x y, 
+     field_mapsto sh t fld x y = 
+               !! (bool_val x (Tpointer t noattr) = Some true) && field_mapsto sh t fld x y.
+Proof.
+intros.
+apply pred_ext; normalize.
+apply andp_right; auto.
+unfold field_mapsto.
+unfold bool_val.
+destruct x; normalize.
+Qed.
+
+Lemma field_offset_exists1: 
+  forall sid t fields fld,
+    type_of_field (unroll_composite_fields sid t fields) fld <> Tvoid ->
+    exists n, field_offset fld fields = Errors.OK n.
+intros.
+unfold field_offset.
+forget 0 as k. revert k.
+induction fields; intro k; simpl in H. congruence.
+destruct (eq_dec i fld). subst i.
+econstructor; simpl. rewrite if_true by auto.
+reflexivity.
+simpl. rewrite if_false by auto.
+destruct (IHfields H (align k (alignof t0) + sizeof t0)).
+eauto.
+Qed.
+
+
+Lemma field_mapsto_access_mode:
+  forall sh v t fld v' id fList att,
+   t = Tstruct id fList att ->
+  field_mapsto sh t fld v v' = 
+   !! (exists ch, access_mode (type_of_field (unroll_composite_fields id t fList) fld) = By_value ch) 
+           && field_mapsto sh t fld v v'.
+Proof.
+intros. subst.
+apply pred_ext; normalize.
+apply andp_right; auto.
+unfold field_mapsto.
+destruct v; normalize.
+destruct (field_offset fld (unroll_composite_fields id (Tstruct id fList att) fList)); normalize.
+case_eq (access_mode
+    (type_of_field
+       (unroll_composite_fields id (Tstruct id fList att) fList) fld)); intros; normalize.
+apply prop_right; eauto.
+Qed.
+
+Import SequentialClight.SeqC.CSL.
+
+
+Lemma splice_top_top: Share.splice Share.top Share.top = Share.top.
+Proof.
+unfold Share.splice.
+unfold Share.Lsh, Share.Rsh.
+case_eq (Share.split Share.top); intros L R ?.
+simpl.
+do 2 rewrite Share.rel_top1.
+erewrite Share.split_together; eauto.
+Qed.
+
+
+(* move this elsewhere, and by the way it generalizes the same-named lemma
+  in veric/semax_straight.v *)
+Lemma cast_exists : forall Delta e2 t rho 
+(TC: typecheck_environ rho Delta = true), 
+denote_tc_assert (typecheck_expr Delta e2) rho ->
+denote_tc_assert (isCastResultType (typeof e2) t t e2)
+  rho ->
+sem_cast (eval_expr e2 rho) (typeof e2) t =
+Some (force_val (sem_cast (eval_expr e2 rho) (typeof e2) t)).
+Proof.
+intros. 
+assert (exists v, sem_cast (eval_expr e2 rho) (typeof e2) t= Some v).
+
+apply expr_lemmas.typecheck_expr_sound in H.
+rename t into t0.
+remember (typeof e2); remember (eval_expr e2 rho). 
+unfold sem_cast. unfold classify_cast.
+Transparent Float.intoffloat.
+Transparent Float.intuoffloat.
+destruct t; destruct v; destruct t0; simpl in *;
+try congruence; try contradiction; eauto;
+try solve [
+unfold Float.intoffloat, Float.intuoffloat; repeat invSome;
+inversion2 H1 H0; hnf in H2,H3; rewrite H3; rewrite Zle_bool_rev; rewrite H2;
+simpl; eauto];
+try solve [
+try destruct i; try destruct s; try destruct i0; try destruct i1; try destruct s0; eauto |
+
+destruct i; destruct s; unfold lift2 in *; try solve[simpl in *; 
+  unfold lift2,lift1 in *;  expr_lemmas.unfold_tc_denote; destruct H0; 
+try rewrite <- Heqv in *; 
+unfold Float.intoffloat; 
+destruct (Float.Zoffloat f0); try contradiction;
+try rewrite H0; try rewrite H1; simpl; eauto | 
+simpl in *;  unfold Float.intuoffloat; destruct H0;
+expr_lemmas.unfold_tc_denote; try rewrite <- Heqv in *; destruct (Float.Zoffloat f0);
+try rewrite H0; try rewrite H1; simpl; eauto; try contradiction] |
+
+try destruct i0; try destruct i1; destruct s; simpl in *; try contradiction; try rewrite H; eauto ].
+
+destruct i; destruct s; unfold lift2 in *;
+simpl in *; unfold lift2,lift1 in *;
+unfold Float.intoffloat, Float.intuoffloat;
+try (
+destruct H0 as [H0 H1]; hnf in H0,H1; rewrite <- Heqv in *;
+destruct (Float.Zoffloat f0); try contradiction;
+hnf in H0,H1; rewrite H0; rewrite expr_lemmas.Zle_bool_rev; rewrite H1;
+simpl; eauto);
+simpl; eauto.
+
+auto.
+Opaque Float.intoffloat.
+Opaque Float.intuoffloat.
+
+destruct H1. rewrite H1. auto.
+Qed. 
+
+(* Admitted:  after Joey checks in his revision of environments,
+ move this definition (and similar ones in progs/assert_lemmas
+  into expr.v, and use it in the definition of eval_expr *)
+Definition eval_cast (t t': type) (v: val) : val := force_val (sem_cast v t t').
+Definition tc_val (t: type) (v: val) : Prop := typecheck_val v t = true.
+
+Lemma typecheck_val_eval_cast: 
+  forall t2 e2 rho Delta,
+      typecheck_environ rho Delta = true ->
+      denote_tc_assert (typecheck_expr Delta e2) rho ->
+      denote_tc_assert (isCastResultType (typeof e2) t2 t2 e2) rho ->
+      typecheck_val (eval_cast (typeof e2) t2 (eval_expr e2 rho)) t2 = true.
+Proof. intros ? ? ? ? H2 H5 H6.
+assert (H7 := cast_exists _ _ _ _ H2 H5 H6).
+assert (H8 := expr_lemmas.typecheck_expr_sound _ _ _ H2 H5).
+clear - H7 H6 H8.
+revert H7; case_eq (sem_cast (eval_expr e2 rho) (typeof e2) t2); intros; inv H7.
+unfold eval_cast. rewrite H. simpl.
+case_eq (eval_expr e2 rho); intros; rename H0 into H99;
+ destruct t2; inv H8; inv H; simpl; auto;
+hnf in H6; try contradiction; rewrite H99 in *;
+destruct (typeof e2); inv H2; inv H1; auto;
+try (unfold sem_cast in H0; simpl in H0;
+      destruct i0; simpl in*; destruct s; inv H0; simpl; auto).
+simpl in *. unfold lift1 in H6. rewrite H99 in *. inv H6. auto.
+simpl in *. unfold isCastResultType in H6. simpl in H6.
+unfold sem_cast in H0. 
+simpl in H0.
+destruct i; simpl in*; destruct s; try destruct f; inv H0; simpl; auto;
+invSome; simpl; auto.
+unfold lift1, denote_tc_iszero in H6; rewrite H99 in *; contradiction.
+unfold lift1, denote_tc_iszero in H6; rewrite H99 in *; contradiction.
+unfold lift1, denote_tc_iszero in H6; rewrite H99 in *; contradiction.
+unfold lift1, denote_tc_iszero in H6; rewrite H99 in *; contradiction.
+unfold lift1, denote_tc_iszero in H6; rewrite H99 in *; contradiction.
+unfold lift1, denote_tc_iszero in H6; rewrite H99 in *; contradiction.
+Qed.
+
+Lemma field_mapsto_offset:
+  forall sh sid fields fld b i v ch,
+  access_mode (type_of_field
+        (unroll_composite_fields sid (Tstruct sid fields noattr) fields) fld) = By_value ch ->        
+  field_mapsto sh (Tstruct sid fields noattr) fld (Vptr b i) v |--
+  match field_offset fld fields with
+  | Errors.OK delta => 
+     address_mapsto ch v (Share.unrel Share.Lsh sh) (Share.unrel Share.Rsh sh)
+            (b, Int.unsigned (Int.add i (Int.repr delta)))
+  | _ => FF
+  end.
+Proof.
+unfold field_mapsto; simpl; intros.
+rewrite H.
+case_eq (field_offset fld
+    (unroll_composite_fields sid (Tstruct sid fields noattr) fields)); intros.
+2: rewrite field_offset_unroll in H0; rewrite H0; auto.
+normalize.
+rewrite field_offset_unroll in H0.
+rewrite H0.
+auto.
+Qed.
+
+Global Opaque field_mapsto.
+
