progs/forward.v
@@ -1,0 +1,436 @@
+Require Import veric.SeparationLogic.
+Require veric.SequentialClight.
+Import SequentialClight.SeqC.CSL.
+Require Import progs.client_lemmas.
+Require Import progs.field_mapsto.
+
+Local Open Scope logic.
+
+
+Lemma semax_load_field:
+forall (Delta: tycontext) (G: funspecs) sh id t1 fld P e1 v2 t2 i2 sid fields ,
+    typeof e1 = Tstruct sid fields noattr ->
+    (temp_types Delta) ! id = Some (t2,i2) ->
+  forall (TC0: t1 = typeof e1) 
+          (TC2: t2 =
+           type_of_field
+             (unroll_composite_fields sid (Tstruct sid fields noattr) fields) fld),
+    semax Delta G 
+       (|> (local (tc_lvalue Delta e1) &&
+          (lift2 (field_mapsto sh t1 fld) (eval_lvalue e1) (lift0 v2) * P)))
+       (Sset id (Efield e1 fld t2))
+       (normal_ret_assert (
+         EX old:val, local (lift1 (eq v2) (eval_id id)) &&
+                  (subst id (lift0 old) 
+                    (lift2 (field_mapsto sh t1 fld) (eval_lvalue e1) (lift0 v2) * P)))).
+Proof with normalize.
+Transparent field_mapsto.
+pose proof I.
+pose proof I.
+intros.
+subst t1.
+rename H2 into TE1.
+apply (semax_pre_post
+            (|> (local (tc_temp Delta id (typeof (Efield e1 fld t2))) &&
+             local (tc_lvalue Delta (Efield e1 fld t2)) &&
+               (mapsto' sh (Efield e1 fld t2) v2 * 
+                  (!! (typecheck_val v2 t2 = true) && !!(type_is_volatile t2 = false) &&  P))))
+            (normal_ret_assert 
+              (EX old:val, local (lift1 (eq v2) (eval_id id)) &&
+              (subst id (lift0 old) (mapsto' sh (Efield e1 fld t2) v2  * 
+                (!! (typecheck_val v2 t2 = true) && !!(type_is_volatile t2 = false) && P))))));
+  [ | | apply semax_load].
+
+(* PRECONDITION *)
+intro rho.
+unfold tc_temp, typecheck_temp_id, local, lift1, lift0.
+simpl. rewrite TE1.
+normalize.
+apply later_derives.
+normalize.
+apply derives_trans with ((!!(eqb_type t2 t2 = true) && !!tc_lvalue Delta (Efield e1 fld t2) rho &&
+    (!!(typecheck_val v2 t2 = true) && !!(type_is_volatile t2 = false) && 
+     (mapsto' sh (Efield e1 fld t2) v2 rho))) * P rho).
+apply sepcon_derives; auto.
+unfold lift2.
+rewrite eqb_type_refl. normalize.
+unfold mapsto'.
+unfold tc_lvalue; simpl. unfold lift2.
+unfold tc_lvalue in H3. rewrite H1.
+unfold field_mapsto.
+case_eq (eval_lvalue e1 rho); intros; normalize.
+rewrite <- TC2.
+rewrite field_offset_unroll.
+case_eq (field_offset fld fields); intros; normalize.
+case_eq (access_mode t2); intros; normalize.
+rewrite H8. 
+normalize.
+normalize.
+
+(* POSTCONDITION *)
+intros ek vl rho; unfold normal_ret_assert; simpl.
+normalize.
+intro old. apply exp_right with old.
+normalize.
+unfold local,lift0,lift1,lift2; simpl.
+normalize.
+unfold subst.
+normalize.
+apply sepcon_derives; auto.
+unfold mapsto', field_mapsto.
+simpl eval_lvalue. simpl typeof.
+case_eq (access_mode t2); intros; normalize.
+destruct (eval_lvalue e1 (env_set rho id old)); normalize.
+rewrite H1.
+rewrite field_offset_unroll.
+destruct (field_offset fld fields); normalize.
+rewrite <- TC2.
+rewrite H4. rewrite H5.
+normalize.
+Opaque field_mapsto.
+Qed.
+
+Lemma semax_store_field: 
+forall (Delta: tycontext) (G: funspecs) e1 fld P v0 t2 e2 sid fields ,
+    typeof e1 = Tstruct sid fields noattr ->
+    t2 = type_of_field
+             (unroll_composite_fields sid (Tstruct sid fields noattr) fields) fld ->
+    typecheck_store (Efield e1 fld t2) ->
+   semax Delta G 
+       (|> (local (tc_lvalue Delta e1) && local (tc_expr Delta (Ecast e2 t2)) &&
+          (lift2 (field_mapsto Share.top (typeof e1) fld) (eval_lvalue e1) v0 * P)))
+       (Sassign (Efield e1 fld t2) e2) 
+       (normal_ret_assert 
+          (lift2 (field_mapsto Share.top (typeof e1) fld) (eval_lvalue e1) 
+                  (lift1 (eval_cast (typeof e2) t2) (eval_expr e2)) * P)).
+Proof.
+Transparent field_mapsto.
+pose proof I.
+intros.
+rename H0 into TE1.
+rename H2 into TCS.
+apply semax_pre with 
+  (EX v':val, 
+    (|>(local (tc_lvalue Delta e1) && local (tc_expr Delta (Ecast e2 t2)) &&
+      (lift2 (field_mapsto Share.top (typeof e1) fld) (eval_lvalue e1) (lift0 v') * P)))).
+apply andp_left2.
+intro rho. simpl. apply exp_right with (v0 rho). auto.
+apply extract_exists_pre; intro v'.
+clear v0. rename v' into v0.
+
+pose proof (semax_store Delta G (Efield e1 fld t2) e2 v0 Share.top 
+               (local (lift1 (tc_val t2) (lift1 (eval_cast (typeof e2) t2) (eval_expr e2))) &&
+                 !! (type_is_volatile t2 = false) &&   P)).
+simpl typeof in H0. rewrite splice_top_top in H0.
+eapply semax_pre_post ; [ | | apply H0; auto].
+apply derives_trans with(|> (local (tc_environ Delta) &&
+  (local (tc_lvalue Delta e1) &&
+   local (tc_expr Delta (Ecast e2 t2)) &&
+   (lift2 (field_mapsto Share.top (typeof e1) fld) (eval_lvalue e1) (lift0 v0) * P)))).
+rewrite (later_andp (local (tc_environ Delta))). apply andp_derives; auto.
+apply now_later.
+apply later_derives.
+intro rho; unfold local,lift0,lift1,lift2. simpl.
+normalize.
+unfold field_mapsto, mapsto'.
+simpl.
+case_eq (eval_lvalue e1 rho); intros; normalize.
+rewrite TE1.
+rewrite field_offset_unroll.
+case_eq (field_offset fld fields); intros; normalize.
+rewrite <- H1. destruct (access_mode t2); normalize.
+apply derives_trans with ((!!tc_lvalue Delta (Efield e1 fld t2) rho &&
+    !!tc_expr Delta (Ecast e2 t2) rho &&
+     (!!tc_val t2 (eval_cast (typeof e2) t2 (eval_expr e2 rho)) &&
+      !!(type_is_volatile t2 = false)) &&
+     address_mapsto m v0 (Share.unrel Share.Lsh Share.top)
+       (Share.unrel Share.Rsh Share.top)
+       (b, Int.unsigned (Int.add i (Int.repr z)))) * P rho).
+apply sepcon_derives; auto. 
+apply andp_right; normalize.
+unfold tc_lvalue; simpl.
+unfold lift2. rewrite TE1.
+repeat apply andp_right; apply prop_right; auto.
+split; auto. split; auto. rewrite H6; auto.
+rewrite H8; simpl; auto.
+eapply typecheck_val_eval_cast; eauto.
+hnf in H4.
+destruct H4; auto.
+unfold tc_expr in H4.
+simpl in H4.
+destruct H4; auto.
+normalize.
+
+intros ek vl rho; unfold local, lift1, normal_ret_assert, lift2; simpl.
+normalize.
+apply sepcon_derives; auto.
+unfold mapsto', field_mapsto.
+simpl.
+case_eq (access_mode t2); intros; normalize.
+case_eq (eval_lvalue e1 rho); intros; normalize.
+rewrite TE1.
+rewrite field_offset_unroll.
+case_eq (field_offset fld fields); intros; normalize.
+rewrite <- H1. rewrite H5.
+normalize.
+Opaque field_mapsto.
+Qed.
+
+Lemma semax_load_field':
+forall (Delta: tycontext) (G: funspecs) sh id t1 fld P Q R e1 v2 t2 i2 sid fields ,
+    t1 = Tstruct sid fields noattr ->
+    typeof e1 = Tpointer t1 noattr ->
+        (temp_types Delta) ! id = Some (t2,i2) ->
+  forall 
+          (TC2: t2 =
+           type_of_field
+             (unroll_composite_fields sid (Tstruct sid fields noattr) fields) fld),
+    semax Delta G 
+       (|> PROPx P (LOCALx (tc_expr Delta e1::Q) (SEPx (lift2 (field_mapsto sh t1 fld) (eval_expr e1) (lift0 v2)::R))))
+       (Sset id (Efield (Ederef e1 t1) fld t2))
+       (normal_ret_assert 
+        (EX old:val,
+          PROPx P (LOCALx (lift1 (eq v2) (eval_id id) :: map (subst id (lift0 old)) Q)
+                (SEPx 
+                  (map (subst id (lift0 old))
+                    (lift2 (field_mapsto sh t1 fld) (eval_expr e1) (lift0 v2) :: R)))))).
+Proof.
+intros.
+eapply semax_pre_post;
+  [ | |  apply (semax_load_field Delta G sh id t1 fld (PROPx P (LOCALx Q (SEPx R))) (Ederef e1 t1)
+   v2 t2 i2 sid fields)].
+match goal with |- ?P |-- _ => 
+ let P' := strip1_later P in apply derives_trans with (|>P' ); [auto 50 with derives | ]
+end.
+apply later_derives.
+go_lower.
+rewrite field_mapsto_nonnull.
+unfold tc_expr, tc_lvalue.
+simpl typecheck_lvalue.
+simpl denote_tc_assert.
+rewrite H0. rewrite H.
+simpl.
+normalize.
+rewrite <- sepcon_andp_prop'.
+apply sepcon_derives; auto.
+unfold bool_val in H6.
+destruct (eval_expr e1 rho); inv H6; normalize.
+
+unfold normal_ret_assert.
+intros ek vl rho; normalize.
+intro old; apply exp_right with old.
+simpl.
+normalize.
+unfold subst.
+unfold lift2.
+unfold PROPx, LOCALx, SEPx.
+simpl.
+normalize.
+case_eq (eval_expr e1 (env_set rho id old)); intros; normalize.
+simpl; auto.
+auto.
+auto.
+auto.
+Qed.
+
+Lemma semax_store_field':
+forall (Delta: tycontext) (G: funspecs) t1 fld P Q R e1 e2 v0 t2 sid fields ,
+    t1 = Tstruct sid fields noattr ->
+    typeof e1 = Tpointer t1 noattr ->
+    t2 = type_of_field (unroll_composite_fields sid (Tstruct sid fields noattr) fields) fld ->
+    typecheck_store (Efield (Ederef e1 t1) fld t2) ->
+    semax Delta G 
+       (|> PROPx P (LOCALx (tc_expr Delta e1::tc_expr Delta (Ecast e2 t2)::Q)
+                             (SEPx (lift2 (field_mapsto Share.top t1 fld) (eval_expr e1) v0::R))))
+       (Sassign (Efield (Ederef e1 t1) fld t2) e2) 
+       (normal_ret_assert
+          (PROPx P (LOCALx Q
+              (SEPx  (lift2 (field_mapsto Share.top t1 fld) (eval_expr e1) 
+                  (lift1 (eval_cast (typeof e2) t2) (eval_expr e2)) :: R))))).
+Proof.
+intros.
+eapply semax_pre_post; [ | | eapply (semax_store_field)].
+3: subst t1; reflexivity.
+3: assumption.
+3: assumption.
+instantiate (2:=v0).
+instantiate (1:=(PROPx P (LOCALx Q (SEPx R)))).
+go_lower. apply later_derives.
+normalize.
+subst t1.
+unfold tc_lvalue.
+rewrite field_mapsto_nonnull.
+normalize.
+unfold bool_val in H.
+revert H; case_eq (eval_expr e1 rho); intros; try discriminate; normalize.
+repeat apply andp_right; normalize.
+simpl.
+unfold lift1, denote_tc_isptr.
+unfold lift2.
+rewrite H.
+normalize.
+rewrite H0; simpl; normalize.
+
+intros ek vl rho; unfold normal_ret_assert, local, lift1, lift2; simpl.
+normalize.
+unfold PROPx, LOCALx; simpl.
+normalize.
+destruct (eval_expr e1 rho); normalize.
+Qed.
+
+Lemma forward_setx:
+  forall Delta G P id e,
+  typecheck_temp_id id (typeof e) Delta = true ->
+  (P |-- local (tc_expr Delta e)) ->
+  semax Delta G
+             P
+             (Sset id e)
+             (normal_ret_assert
+                  (EX old:val,  local (lift2 eq (eval_id id) (subst id (lift0 old) (eval_expr e))) &&
+                            subst id (lift0 old) P)).
+Proof.
+intros.
+eapply semax_pre_post; [ | | apply (semax_set_forward Delta G P id e)].
+eapply derives_trans ; [ | apply now_later].
+go_lower.
+apply andp_right; auto.
+apply H0.
+intros ek vl rho; unfold normal_ret_assert. simpl; normalize.
+intros old ?; apply exp_right with old.
+normalize.
+Qed.
+
+Ltac normalizex :=
+  normalize;
+  repeat 
+  (first [ simpl_tc_expr
+         | flatten_sepcon_in_SEP
+          | apply semax_extract_PROP_True; [solve [auto] | ]
+          | apply semax_extract_PROP; intro
+         | extract_prop_in_LOCAL
+         | extract_exists_in_SEP
+         ]; cbv beta; normalize).
+
+Ltac forward_setx := 
+  first [eapply semax_seq; 
+            [ apply sequential' ; apply forward_setx; [reflexivity | normalizex]
+              | apply extract_exists_pre; normalize; try (intros _) ]
+         | eapply semax_post;  [ | apply forward_setx; [reflexivity | normalizex]];
+            cbv beta; normalize
+        ].
+
+Ltac semax_field_tac1 := 
+   eapply semax_load_field'; 
+     [ reflexivity 
+     | reflexivity 
+     | simpl; reflexivity 
+     | type_of_field_tac ].
+
+Ltac isolate_field_tac e fld R := 
+  match R with 
+     | context [|> lift2 (field_mapsto ?sh ?struct fld) ?e' ?v :: ?R'] =>
+          let n := length_of R in let n' := length_of R' 
+             in rewrite (grab_nth_SEP (n- S n')); simpl minus; unfold nth, delete_nth; normalize;
+                replace e' with (eval_expr e) by auto
+     | context [ lift2 (field_mapsto ?sh ?struct fld) ?e' ?v  :: ?R'] =>
+          let n := length_of R in let n' := length_of R' 
+             in rewrite (grab_nth_SEP (n- S n')); simpl minus; unfold nth, delete_nth; normalize;
+                replace e' with (eval_expr e) by auto
+     end.
+
+Ltac hoist_later_in_pre :=
+     match goal with |- semax _ _ ?P _ _ =>
+       let P' := strip1_later P in apply semax_pre0 with (|> P'); [solve [auto 50 with derives] | ]
+     end.
+
+
+Ltac semax_field_tac :=
+match goal with
+ | |- semax ?Delta _ (PROPx ?P (LOCALx ?Q (SEPx ?R)))
+                  (Ssequence (Sset _ (Efield (Ederef ?e _) ?fld _)) _) _ =>
+  apply (semax_pre (PROPx P (LOCALx (tc_expr Delta e :: Q) (SEPx R))));
+   [ go_lower 
+   | isolate_field_tac e fld R; hoist_later_in_pre;
+     eapply semax_seq; [ apply sequential'; semax_field_tac1  
+                                          | simpl update_tycon; apply extract_exists_pre
+                                          ]
+    ]
+ | |- semax ?Delta _ (PROPx ?P (LOCALx ?Q (SEPx ?R)))
+                    (Sset _ (Efield (Ederef ?e _) ?fld _)) _ =>
+     apply (semax_pre (PROPx P (LOCALx (tc_expr Delta e :: Q) (SEPx R))));
+     [ go_lower 
+     | isolate_field_tac e fld R; hoist_later_in_pre;
+       eapply semax_post; [ | semax_field_tac1]
+     ]
+end; normalizex.
+
+
+Ltac store_field_tac1 := 
+  eapply semax_store_field'; [ reflexivity | reflexivity | type_of_field_tac |
+               try solve [hnf; intuition] ].
+
+Ltac store_field_tac :=
+  match goal with
+  | |- semax ?Delta _ (PROPx ?P (LOCALx ?Q (SEPx ?R))) 
+                     (Ssequence (Sassign (Efield (Ederef ?e _) ?fld ?t2) ?e2) _) _ =>
+       apply (semax_pre (PROPx P 
+                (LOCALx (tc_expr Delta e :: tc_expr Delta (Ecast e2 t2) ::Q) 
+                (SEPx R))));
+   [ unfold tc_expr; go_lower 
+   | isolate_field_tac e fld R; hoist_later_in_pre;
+      eapply semax_seq; [ apply sequential'; store_field_tac1   |  ]
+   ]
+  | |- semax ?Delta _ (PROPx ?P (LOCALx ?Q (SEPx ?R))) 
+                     (Sassign (Efield (Ederef ?e _) ?fld ?t2) ?e2) _ =>
+       apply (semax_pre (PROPx P 
+                (LOCALx (tc_expr Delta e :: tc_expr Delta (Ecast e2 t2) ::Q) 
+                (SEPx R))));
+   [ unfold tc_expr; go_lower 
+   | isolate_field_tac e fld R; hoist_later_in_pre;
+       eapply semax_post; [ | store_field_tac1]
+   ]
+  end.
+
+Ltac check_sequential s :=
+ match s with
+ | Sskip => idtac
+ | Sassign _ _ => idtac
+ | Sset _ _ => idtac
+ | Scall _ _ _ => idtac
+ | Ssequence ?s1 ?s2 => check_sequential s1; check_sequential s2
+ | _ => fail
+ end.
+
+Ltac sequential := 
+ match goal with
+ |  |- semax _ _ _ _ (normal_ret_assert _) => fail 2
+ |  |- semax _ _ _ ?s _ =>  check_sequential s; apply sequential
+ end.
+
+Ltac is_canonical P :=
+ match P with 
+ | PROPx _ (LOCALx _ (SEPx _)) => idtac
+ | _ => fail 2 "precondition is not canonical (PROP _ LOCAL _ SEP _)"
+ end.
+
+Ltac forward := 
+  match goal with
+  | |- semax _ _ ?P (Ssequence (Sassign (Efield _ _ _) _) _) _ => 
+                  is_canonical P; store_field_tac
+  | |- semax _ _ ?P (Sassign (Efield _ _ _) _) _ => 
+                  is_canonical P; store_field_tac
+  | |- semax _ _ ?P (Ssequence (Sset _ (Efield _ _ _)) _) _ => 
+                  is_canonical P; semax_field_tac
+  | |- semax _ _ ?P (Sset _ (Efield _ _ _)) _ => 
+                  is_canonical P; semax_field_tac
+  | |- semax _ _ ?P (Ssequence (Sset _ ?e) _) _ => 
+               is_canonical P; match e with (Efield _ _ _) => fail 2 | _ => forward_setx end
+  | |- semax _ _ ?P (Sset _ ?e) _ => 
+               is_canonical P; match e with (Efield _ _ _) => fail 2 | _ => forward_setx end
+  | |- semax _ _ _ (Ssequence (Sreturn _) _) _ =>
+          apply semax_seq with FF; [eapply semax_pre; [ | apply semax_return ]
+                                | apply semax_ff]
+  | |- semax _ _ _ (Sreturn _) _ =>
+          eapply semax_pre; [ | apply semax_return ]
+  end.
+
